IronFleetDefault/ironfleet/src/Dafny/Distributed/Protocol/CausalMesh/proof/assumptions.dfy
@@ -7,6 +7,7 @@ import opened CausalMesh_Message_i
 import opened CausalMesh_Types_i
 import opened Environment_s
 import opened CausalMesh_DistributedSystem_i
+import opened CausalMesh_Properties_i
 import opened Temporal__Temporal_s
 import opened Collections__Maps2_s
 
