IronFleetDefault/ironfleet/src/Dafny/Distributed/Protocol/CausalMesh/properties.dfy
@@ -1,0 +1,71 @@
+include "../../Common/Collections/Maps.i.dfy"
+include "types.dfy"
+include "message.dfy"
+
+module CausalMesh_Properties_i {
+    import opened Collections__Maps_i
+    import opened CausalMesh_Types_i
+    import opened CausalMesh_Message_i
+    
+    /** Key Properties */
+
+    predicate CausalCut(ccache: CCache)
+        // requires CCacheValid(ccache)
+        requires forall k :: k in ccache ==> MetaValid(ccache[k])
+    {
+        forall k :: k in ccache ==>
+            forall kk :: kk in ccache[k].deps ==>
+                kk in ccache &&
+                (VCHappendsBefore(ccache[k].deps[kk], ccache[kk].vc) || VCEq(ccache[k].deps[kk], ccache[kk].vc))
+    }
+
+    predicate ReadsDepsAreMet2(icache:ICache, ccache:CCache, deps:Dependency)
+        requires ICacheValid(icache)
+        requires CCacheValid(ccache)
+        requires forall k :: k in Keys_domain ==> k in icache && k in ccache
+        requires DependencyValid(deps)
+    {
+        forall k :: k in deps ==> 
+            var m := FoldMetaSet(ccache[k], icache[k], icache.Keys);
+            VCEq(deps[k], m.vc) || VCHappendsBefore(deps[k], m.vc)
+    }
+
+    predicate ReadsDepsAreMet(icache:ICache, ccache:CCache, deps:Dependency)
+        requires ICacheValid(icache)
+        requires CCacheValid(ccache)
+        requires forall k :: k in Keys_domain ==> k in icache && k in ccache
+        requires DependencyValid(deps)
+    {
+        forall k :: k in deps ==> 
+            (VCEq(deps[k], ccache[k].vc) || VCHappendsBefore(deps[k], ccache[k].vc))
+            || exists m :: m in icache[k] && m.vc == deps[k]
+            // var m := FoldMetaSet(ccache[k], icache[k], icache.Keys);
+            // VCEq(deps[k], m.vc) || VCHappendsBefore(deps[k], m.vc)
+    }
+
+    predicate UponReadsDepsAreMet(ccache:CCache, deps:Dependency)
+        requires CCacheValid(ccache)
+        requires forall k :: k in Keys_domain ==> k in ccache
+        requires DependencyValid(deps)
+    {
+        forall k :: k in deps ==> 
+            VCEq(deps[k], ccache[k].vc) || VCHappendsBefore(deps[k], ccache[k].vc)
+    }
+    
+    lemma lemma_MergeCCacheRemainsCausalCut(c1:CCache, c2:CCache)
+        requires CCacheValid(c1)
+        requires CCacheValid(c2)
+        requires CausalCut(c1)
+        requires CausalCut(c2)
+        ensures CCacheValid(MergeCCache(c1,c2))
+        ensures CausalCut(MergeCCache(c1,c2))
+    {
+        // map k | k in c1.Keys + c2.Keys ::
+        //     if k in c1 && k in c2 then
+        //         MetaMerge(c1[k], c2[k])
+        //     else if k in c1 then
+        //         c1[k]
+        //     else
+        //         c2[k]
+    }
+}
